proof/Isolation/ConsistencyProperties.v
@@ -1,46 +1,10 @@
-(*******************************************************************************)
-(*  © Université de Lille, The Pip Development Team (2015-2021)                *)
-(*                                                                             *)
-(*  This software is a computer program whose purpose is to run a minimal,     *)
-(*  hypervisor relying on proven properties such as memory isolation.          *)
-(*                                                                             *)
-(*  This software is governed by the CeCILL license under French law and       *)
-(*  abiding by the rules of distribution of free software.  You can  use,      *)
-(*  modify and/ or redistribute the software under the terms of the CeCILL     *)
-(*  license as circulated by CEA, CNRS and INRIA at the following URL          *)
-(*  "http://www.cecill.info".                                                  *)
-(*                                                                             *)
-(*  As a counterpart to the access to the source code and  rights to copy,     *)
-(*  modify and redistribute granted by the license, users are provided only    *)
-(*  with a limited warranty  and the software's author,  the holder of the     *)
-(*  economic rights,  and the successive licensors  have only  limited         *)
-(*  liability.                                                                 *)
-(*                                                                             *)
-(*  In this respect, the user's attention is drawn to the risks associated     *)
-(*  with loading,  using,  modifying and/or developing or reproducing the      *)
-(*  software by the user in light of its specific status of free software,     *)
-(*  that may mean  that it is complicated to manipulate,  and  that  also      *)
-(*  therefore means  that it is reserved for developers  and  experienced      *)
-(*  professionals having in-depth computer knowledge. Users are therefore      *)
-(*  encouraged to load and test the software's suitability as regards their    *)
-(*  requirements in conditions enabling the security of their systems and/or   *)
-(*  data to be ensured and,  more generally, to use and operate it in the      *)
-(*  same conditions as regards security.                                       *)
-(*                                                                             *)
-(*  The fact that you are presently reading this means that you have had       *)
-(*  knowledge of the CeCILL license and that you accept its terms.             *)
-(*******************************************************************************)
+From Pip.Model.Isolation Require Import IsolationTypes IsolationState IsolationInterface.
+From Pip.Proof.Isolation Require Import ModelExclusiveFunctions.
 
+Require Import List.
 
-(** * Summary 
-    This file contains the formalization of the consistency properties : 
-for each one we summarize the description of its definition *)
-Require Import Pip.Model.ADT Pip.Model.Hardware Pip.Model.MAL Pip.Model.Lib.
-
-Require Import Pip.Proof.Lib Pip.Proof.Isolation Pip.Proof.StateLib.
-
-Require Import List Coq.Logic.ProofIrrelevance.
-Import List.ListNotations.
+Import IsolationTypes.
+Import IsolationState.
 
 (** ** The [dataStructurePdSh1Sh2asRoot] property defines the type of different values 
 stored into the page directory structure, the first shadow structure and 
@@ -54,89 +18,68 @@ Configuation tables of the last level must contain :
   data structure
 The other tables contain Physical entries  
     [idxroot] should be PDidx, sh1idx or sh2idx.
- (1)   
+ (1)
 *)
 Definition dataStructurePdSh1Sh2asRoot (idxroot : index) (s : state) :=
-forall (partition : page),  
-In partition (getPartitions pageRootPartition s) -> 
-forall entry, nextEntryIsPP partition idxroot entry s ->  
-forall va : vaddr, 
-True -> forall level stop , Some level = getNbLevel -> 
-forall indirection idx, getIndirection entry va level stop s = Some indirection -> 
-( indirection = pageDefault \/ 
-(( ( stop < level /\ isPE indirection idx s )\/  
-   ( stop >= level /\ ( (isVE indirection idx s /\ idxroot = idxShadow1) \/ 
-                       (isVA indirection idx s /\ idxroot = idxShadow2) \/ 
-                       (isPE indirection idx s /\ idxroot = idxPageDir) ) ))
-                       /\ 
-  indirection <> pageDefault)) .
+forall (partition : page), In partition (getPartitions pageRootPartition s) ->
+forall entry, nextEntryIsPP partition idxroot entry s ->
+forall va : vaddr, forall level stop, Some level = getNbLevel ->
+forall indirection idx, getIndirection entry va level stop s = Some indirection ->
+( indirection = pageDefault \/
+  ( ( ( stop < level  /\ isPE indirection idx s) \/
+      ( stop >= level /\ ( (isVE indirection idx s /\ idxroot = idxShadow1) \/
+                           (isVA indirection idx s /\ idxroot = idxShadow2) \/
+                           (isPE indirection idx s /\ idxroot = idxPageDir))))
+    /\ indirection <> pageDefault)
+).
 
 Definition wellFormedFstShadow (s : state) :=
-forall partition,
-In partition (getPartitions pageRootPartition s) -> 
-forall va pg pd sh1,
-StateLib.getPd partition (memory s) = Some pd -> 
-StateLib.getFstShadow partition (memory s) = Some sh1 ->
-getMappedPage pd s va= SomePage pg ->       
-exists vainparent, getVirtualAddressSh1 sh1 s va = Some vainparent. 
+forall partition, In partition (getPartitions pageRootPartition s) ->
+forall va pg pd sh1, getPd partition (memory s) = Some pd ->
+getFstShadow partition (memory s) = Some sh1 ->
+getMappedPage pd s va = SomePage pg ->
+exists vainparent, getVirtualAddressSh1 sh1 s va = Some vainparent.
 
 Definition wellFormedSndShadow (s : state) :=
-forall partition,
-In partition (getPartitions pageRootPartition s) -> 
+forall partition, In partition (getPartitions pageRootPartition s) ->
 partition <> pageRootPartition ->
-forall va pg pd sh2,
-StateLib.getPd partition (memory s) = Some pd ->
-StateLib.getSndShadow partition (memory s) = Some sh2 ->
-getMappedPage pd s va= SomePage pg ->
+forall va pg pd sh2, getPd partition (memory s) = Some pd ->
+getSndShadow partition (memory s) = Some sh2 ->
+getMappedPage pd s va = SomePage pg ->
 exists vainparent, getVirtualAddressSh2 sh2 s va = Some vainparent /\
-vaddrEq vaddrDefault vainparent = false .
+vaddrEq vaddrDefault vainparent = false.
 
 Definition wellFormedShadows (idxroot : index) (s : state) :=
-forall (partition : page),
-In partition (getPartitions pageRootPartition s) ->
-forall pdroot ,
-StateLib.getPd partition (memory s) = Some pdroot ->
+forall (partition : page), In partition (getPartitions pageRootPartition s) ->
+forall pdroot, getPd partition (memory s) = Some pdroot ->
 forall structroot, nextEntryIsPP partition idxroot structroot s ->
-forall nbL stop , Some nbL = getNbLevel ->
-forall indirection1  va b,
-getIndirection pdroot va nbL stop s = Some indirection1 ->
+forall nbL stop, Some nbL = getNbLevel ->
+forall indirection1 va b, getIndirection pdroot va nbL stop s = Some indirection1 ->
 (Nat.eqb pageDefault indirection1) = b ->
-(exists indirection2,
-getIndirection structroot va nbL stop s = Some indirection2 /\
+(exists indirection2, getIndirection structroot va nbL stop s = Some indirection2 /\
 (Nat.eqb pageDefault indirection2) = b).
-
-(* Definition fstShadowWellFormed (s : state) :=
-forall (partition : page),  
-In partition (getPartitions multiplexer s) -> 
-forall pdroot sh1Root, 
-StateLib.getPd partition (memory s) = Some pdRoot -> 
-StateLib.getFstShadow partition (memory s) = Some sh1Root ->
-forall level stop , Some level = getNbLevel -> 
-forall indirection1 indirection2 va, 
-getIndirection pdRoot va level stop s = Some defaultPage ->
-getIndirection sh1Root va level stop s = Some defaultPage.  *)
 
 (** ** The [currentPartitionInPartitionsList] property specifies that the 
     current partition must be into the list of partitions retrieved from the 
     first created partition (multiplexer) 
     (2) *)
-Definition currentPartitionInPartitionsList (s : state) := 
- In (currentPartition s) (getPartitions pageRootPartition s).
+Definition currentPartitionInPartitionsList (s : state) :=
+In (currentPartition s) (getPartitions pageRootPartition s).
 
 (** ** The [currentPartitionIsNotDefaultPage t] property specifies that the 
     current partition is not a default physical page  
     (2) *)
 Definition currentPartitionIsNotDefaultPage (s : state) :=
- (currentPartition s) <> pageDefault. 
- 
+(currentPartition s) <> pageDefault.
+
 (** ** The [parentInPartitionList] property specifies that the parent of a given 
 partition should be into the list of partitions retrieved from the 
     first created partition (multiplexer) 
     (3) *)
-Definition parentInPartitionList (s : state) := 
-forall partition, In partition (getPartitions pageRootPartition s) -> 
+Definition parentInPartitionList (s : state) :=
+forall partition, In partition (getPartitions pageRootPartition s) ->
 forall parent, nextEntryIsPP partition idxParentDesc parent s ->
-In parent (getPartitions pageRootPartition s). 
+In parent (getPartitions pageRootPartition s).
 
 (** ** The [partitionDescriptorEntry] defines some properties of the partition descriptor. 
     - A partition descriptor is a table containing virtual addresses and physical pages.
@@ -145,15 +88,17 @@ In parent (getPartitions pageRootPartition s).
     - The successors of these indices contain physical pages which should not be 
       equal to "defaultPage".
     (4) *)
-Definition partitionDescriptorEntry s := 
-forall (partition : page),  
-In partition (getPartitions pageRootPartition s) -> 
-forall (idxroot : index), (idxroot = idxPageDir \/ idxroot = idxShadow1 \/ idxroot = idxShadow2 \/ 
-idxroot = idxShadow3 \/
-idxroot = idxParentDesc  \/ idxroot = idxPartDesc ) ->
-idxroot < tableSize - 1  /\
-isVA partition idxroot  s /\ 
-exists entry, nextEntryIsPP partition idxroot entry s  /\  
+Definition partitionDescriptorEntry s :=
+forall (partition : page), In partition (getPartitions pageRootPartition s) ->
+forall (idxroot : index), (idxroot = idxPageDir \/
+                           idxroot = idxShadow1 \/
+                           idxroot = idxShadow2 \/
+                           idxroot = idxShadow3 \/
+                           idxroot = idxParentDesc \/
+                           idxroot = idxPartDesc) ->
+idxroot < tableSize - 1 /\
+isVA partition idxroot s /\
+exists entry, nextEntryIsPP partition idxroot entry s /\
 entry <> pageDefault.
 
 (** ** The [multiplexerWithoutParent] specifies that the multiplexer is the root of
@@ -165,195 +110,171 @@ getParent pageRootPartition (memory s) = None.
     are different 
     (5) *)
 Definition noDupMappedPagesList s :=
-forall (partition : page),  
-In partition (getPartitions pageRootPartition s) ->  
- NoDup ((getMappedPages partition s)).
- 
+forall (partition : page), In partition (getPartitions pageRootPartition s) ->
+NoDup ((getMappedPages partition s)).
+
 (** ** The [noDupConfigPagesList] requires that configuation tables of
     a single partition are different 
     (6) *)
 Definition noDupConfigPagesList s :=
-forall (partition : page),  
-In partition (getPartitions pageRootPartition s) -> 
+forall (partition : page), In partition (getPartitions pageRootPartition s) ->
 NoDup (getConfigPages partition s).
-(* forall root, nextEntryIsPP partition idxroot root s->
- NoDup (getIndirections root s). 
- *)
+
 (** ** The [accessibleVAIsNotPartitionDescriptor] requires that accessible virtual 
     addresses are not marked as partition descriptor into the first shadow configuation
     structure 
     (7) *)
 Definition accessibleVAIsNotPartitionDescriptor s :=
-forall partition va pd sh1 page, 
-  In partition (getPartitions pageRootPartition s) -> 
-  StateLib.getPd partition (memory s) = Some pd -> 
-  StateLib.getFstShadow partition (memory s) = Some sh1 -> 
-  getAccessibleMappedPage pd s va = SomePage page -> 
-  getPDFlag sh1 va s = false.
+forall partition va pd sh1 page, In partition (getPartitions pageRootPartition s) ->
+getPd partition (memory s) = Some pd ->
+getFstShadow partition (memory s) = Some sh1 ->
+getAccessibleMappedPage pd s va = SomePage page ->
+getPDFlag sh1 va s = false.
 
 (** ** The [accessibleChildPageIsAccessibleIntoParent] requires that all accessible physical 
       pages into a given partition should be accessible into its parent
     (8) *)
-Definition  accessibleChildPageIsAccessibleIntoParent s := 
-forall partition va pd  accessiblePage, 
-  In partition (getPartitions pageRootPartition s) ->
-  StateLib.getPd partition (memory s) = Some pd ->
-  getAccessibleMappedPage pd s va = SomePage accessiblePage ->
-  isAccessibleMappedPageInParent partition va accessiblePage s = true. 
+Definition  accessibleChildPageIsAccessibleIntoParent s :=
+forall partition va pd accessiblePage, In partition (getPartitions pageRootPartition s) ->
+getPd partition (memory s) = Some pd ->
+getAccessibleMappedPage pd s va = SomePage accessiblePage ->
+isAccessibleMappedPageInParent partition va accessiblePage s = true.
 
 (** ** The [noCycleInPartitionTree] requires that a partition and 
-        its ancestors are different 
+        its ancestors are different
     (9) **)
-Definition noCycleInPartitionTree s := 
-forall ancestor partition, 
-In partition (getPartitions pageRootPartition s) -> 
-In ancestor (getAncestors partition s) -> 
+Definition noCycleInPartitionTree s :=
+forall ancestor partition, In partition (getPartitions pageRootPartition s) ->
+In ancestor (getAncestors partition s) ->
 ancestor <> partition.
 
 (** ** The [configTablesAreDifferent] requires that configuation tables of different
         partitions are disjoint
       (10) **)
-Definition configTablesAreDifferent s := 
-forall partition1 partition2,
-In partition1 (getPartitions pageRootPartition s) -> 
-In partition2 (getPartitions pageRootPartition s) -> 
-partition1 <> partition2 -> 
+Definition configTablesAreDifferent s :=
+forall partition1 partition2, In partition1 (getPartitions pageRootPartition s) ->
+In partition2 (getPartitions pageRootPartition s) ->
+partition1 <> partition2 ->
 disjoint (getConfigPages partition1 s) (getConfigPages partition2 s).
 
 (** ** The [isChild] specifies that a given partition should be a child of the 
         physical page stored as parent into the associated partition descriptor 
     (11) **)
-Definition isChild  s :=
-forall partition parent : page,
-In partition (getPartitions pageRootPartition s) -> 
-StateLib.getParent partition (memory s) = Some parent -> 
+Definition isChild s :=
+forall partition parent : page, In partition (getPartitions pageRootPartition s) ->
+getParent partition (memory s) = Some parent ->
 In partition (getChildren parent s).
-
 
 (** ** The [isParent] specifies that if we take any child into the children list of any 
 partition into the partition list so this partition should be the parent of this child 
  (..) **)
-Definition isParent  s :=
-forall partition parent : page,
-In parent (getPartitions pageRootPartition s) -> 
-In partition (getChildren parent s) -> 
-StateLib.getParent partition (memory s) = Some parent.
+Definition isParent s :=
+forall partition parent : page, In parent (getPartitions pageRootPartition s) ->
+In partition (getChildren parent s) ->
+getParent partition (memory s) = Some parent.
 
 (** ** The [isPresentNotDefaultIff] specifies that if the present flag of a physical 
     entry is equal to false so the associated physical page must be equal to the default 
     value 
     (12) **)
-Definition isPresentNotDefaultIff s:=
-forall table idx , 
- readPresent table idx (memory s) = Some false <-> 
- readPhyEntry table idx (memory s) = Some pageDefault .
+Definition isPresentNotDefaultIff s :=
+forall table idx,
+readPresent table idx (memory s) = Some false <->
+readPhyEntry table idx (memory s) = Some pageDefault.
 
 (** ** The [physicalPageNotDerived] specifies that if a given physical
     page is marked as not derived in a parent so it is not mapped in any child
     (13)
-**) 
-Definition physicalPageNotDerived s := 
-forall parent va pdParent pageParent, 
-In parent (getPartitions pageRootPartition s) -> 
-StateLib.getPd parent (memory s) = Some pdParent -> 
-~ isDerived parent va s -> 
-getMappedPage pdParent s va = SomePage pageParent -> 
-forall child pdChild vaInChild pageChild , 
-In child (getChildren parent s) -> 
-StateLib.getPd child (memory s) = Some pdChild -> 
-getMappedPage pdChild s vaInChild = SomePage  pageChild -> 
+**)
+Definition physicalPageNotDerived s :=
+forall parent va pdParent pageParent, In parent (getPartitions pageRootPartition s) ->
+getPd parent (memory s) = Some pdParent ->
+~isDerived parent va s ->
+getMappedPage pdParent s va = SomePage pageParent ->
+forall child pdChild vaInChild pageChild, In child (getChildren parent s) ->
+getPd child (memory s) = Some pdChild ->
+getMappedPage pdChild s vaInChild = SomePage  pageChild ->
 pageParent <> pageChild.
 
 Definition noDupPartitionTree s :=
-NoDup (getPartitions pageRootPartition s) .
-
+NoDup (getPartitions pageRootPartition s).
 
 Definition wellFormedFstShadowIfDefaultValues s :=
-forall partition va pd sh1 , 
-In partition (getPartitions pageRootPartition s) -> 
-StateLib.getPd partition (memory s) = Some pd -> 
-StateLib.getFstShadow partition (memory s) = Some sh1 -> 
-getMappedPage pd s va = SomeDefault-> 
-getPDFlag sh1 va s = false /\ 
+forall partition va pd sh1, In partition (getPartitions pageRootPartition s) ->
+getPd partition (memory s) = Some pd ->
+getFstShadow partition (memory s) = Some sh1 ->
+getMappedPage pd s va = SomeDefault->
+getPDFlag sh1 va s = false /\
 getVirtualAddressSh1 sh1 s va = Some vaddrDefault.
 
 Definition wellFormedFstShadowIfNone s :=
-forall partition va pd sh1 , 
-In partition (getPartitions pageRootPartition s) -> 
-StateLib.getPd partition (memory s) = Some pd -> 
-StateLib.getFstShadow partition (memory s) = Some sh1 -> 
-getMappedPage pd s va =  NonePage -> 
-getPDFlag sh1 va s = false /\ 
+forall partition va pd sh1,
+In partition (getPartitions pageRootPartition s) ->
+getPd partition (memory s) = Some pd ->
+getFstShadow partition (memory s) = Some sh1 ->
+getMappedPage pd s va =  NonePage ->
+getPDFlag sh1 va s = false /\
 getVirtualAddressSh1 sh1 s va = None.
 
-
 (** Consistency : Linked list properties **)
-Definition LLconfiguration1 s:=
-forall part fstLL LLtable,
-In part (getPartitions pageRootPartition s) -> 
-nextEntryIsPP part idxShadow3 fstLL s ->  
-In LLtable (getLLPages part s nbPage) -> 
+Definition LLconfiguration1 s :=
+forall part fstLL LLtable, In part (getPartitions pageRootPartition s) -> 
+nextEntryIsPP part idxShadow3 fstLL s ->
+In LLtable (getLLPages part s nbPage) ->
 isI LLtable (CIndex 1) s.
 
-
-Definition LLconfiguration2 s:=
-forall part fstLL LLtable maxidx,
-In part (getPartitions pageRootPartition s) -> 
-nextEntryIsPP part idxShadow3 fstLL s ->  
-In LLtable (getLLPages part s nbPage) -> 
-StateLib.getMaxIndex = Some maxidx -> 
+Definition LLconfiguration2 s :=
+forall part fstLL LLtable maxidx, In part (getPartitions pageRootPartition s) ->
+nextEntryIsPP part idxShadow3 fstLL s ->
+In LLtable (getLLPages part s nbPage) ->
+getMaxIndex = Some maxidx ->
 isPP LLtable maxidx s.
 
-Definition LLconfiguration3 s:=
-forall part fstLL LLtable,
-In part (getPartitions pageRootPartition s) -> 
-nextEntryIsPP part idxShadow3 fstLL s ->  
-In LLtable (getLLPages part s (nbPage+1)) -> 
+Definition LLconfiguration3 s :=
+forall part fstLL LLtable, In part (getPartitions pageRootPartition s) ->
+nextEntryIsPP part idxShadow3 fstLL s ->
+In LLtable (getLLPages part s (nbPage+1)) ->
 isI LLtable (CIndex 0) s.
 
-Definition LLconfiguration4 s:=
-forall part fstLL LLtable,
-In part (getPartitions pageRootPartition s) -> 
-nextEntryIsPP part idxShadow3 fstLL s ->  
-In LLtable (getLLPages part s (nbPage+1)) -> 
-exists FFI nextFFI,
-StateLib.readIndex LLtable (CIndex 0) (memory s)= Some FFI 
-/\ isVA LLtable FFI s /\ FFI < tableSize - 1 
-/\ StateLib.Index.succ FFI = Some nextFFI
+Definition LLconfiguration4 s :=
+forall part fstLL LLtable, In part (getPartitions pageRootPartition s) ->
+nextEntryIsPP part idxShadow3 fstLL s ->
+In LLtable (getLLPages part s (nbPage+1)) ->
+exists FFI nextFFI, readIndex LLtable (CIndex 0) (memory s) = Some FFI
+/\ isVA LLtable FFI s
+/\ FFI < tableSize - 1
+/\ Index.succ FFI = Some nextFFI
 /\ isI LLtable nextFFI s.
 
 Definition LLconfiguration5 s:=
-forall part fstLL ,
-In part (getPartitions pageRootPartition s) -> 
-nextEntryIsPP part idxShadow3 fstLL s ->  
+forall part fstLL, In part (getPartitions pageRootPartition s) ->
+nextEntryIsPP part idxShadow3 fstLL s ->
 NoDup (getLLPages fstLL s (nbPage + 1)).
 
-Definition LLconfiguration5' s:=
-forall partition LL LLtable FFI nextFFI, 
-In partition (getPartitions pageRootPartition s) ->
+Definition LLconfiguration5' s :=
+forall partition LL LLtable FFI nextFFI, In partition (getPartitions pageRootPartition s) ->
 getConfigTablesLinkedList partition (memory s) = Some LL ->
 In LLtable (getLLPages LL s (nbPage + 1)) ->
 isIndexValue LLtable (CIndex 0) FFI s ->
-StateLib.Index.succ FFI = Some nextFFI ->
-StateLib.getMaxIndex <> Some nextFFI /\ 
-nextFFI <> CIndex 1. 
+Index.succ FFI = Some nextFFI ->
+getMaxIndex <> Some nextFFI /\ nextFFI <> CIndex 1.
 
 
 (*%%%%%%%%%%%%%%%%%%%%%%%%%%%%%%%%%%%%%%%%%%%%%%%%%%%%%%%%%%*)
 (** ** Conjunction of all consistency properties *)
-Definition consistency s := 
- partitionDescriptorEntry s /\  
+Definition consistency s :=
+ partitionDescriptorEntry s /\
  dataStructurePdSh1Sh2asRoot idxPageDir s /\
  dataStructurePdSh1Sh2asRoot idxShadow1 s /\
  dataStructurePdSh1Sh2asRoot idxShadow2 s /\
  currentPartitionInPartitionsList s /\
  noDupMappedPagesList s /\
- noDupConfigPagesList s  /\
+ noDupConfigPagesList s /\
  parentInPartitionList s /\
  accessibleVAIsNotPartitionDescriptor s /\
  accessibleChildPageIsAccessibleIntoParent s /\
- noCycleInPartitionTree s /\ 
- configTablesAreDifferent s /\ 
+ noCycleInPartitionTree s /\
+ configTablesAreDifferent s /\
  isChild s /\
  isPresentNotDefaultIff s /\
  physicalPageNotDerived s /\
