proof/Isolation/IsolationProperties.v
@@ -1,40 +1,28 @@
-(* From Pip.Model.Meta Require Import TypesModel StateModel StateAgnosticMonad InterfaceModel. *)
 From Pip.Model.Isolation Require Import IsolationTypes IsolationState IsolationInterface.
+From Pip.Proof.Isolation Require Import ModelExclusiveFunctions.
 
 Require Import List.
 
 Import IsolationTypes.
 
-(* Require Import Pip.Model.ADT Pip.Model.Hardware Pip.Model.Lib Pip.Model.MAL. *)
-(* Require Import Pip.Proof.Isolation StateLib Pip.Proof.Lib. *)
-
-(* Import List.ListNotations. *)
-
 (** THE VERTICAL SHARING PROPERTY:
     All child used pages (configuration tables and mapped pages) are mapped into 
     the parent partition  *)
 Definition verticalSharing s : Prop :=
-
 forall parent child : page,
   In parent (getPartitions pageRootPartition s) ->
   In child (getChildren parent s) ->
   incl (getUsedPages child s) (getMappedPages parent s).
 
-(** THE ISOLATION PROPERTY BETWEEN PARTITIONS, 
-    If we take two different children of a given parent, 
+(** THE ISOLATION PROPERTY BETWEEN PARTITIONS,
+    If we take two different children of a given parent,
     so all their used pages are different  *)
-Definition partitionsIsolation  s : Prop :=  
-
-forall parent child1 child2 : page , 
-
-  In parent (getPartitions pageRootPartition s)-> 
-
-  In child1 (getChildren parent s) -> 
-
-  In child2 (getChildren parent s) -> 
-
+Definition partitionsIsolation  s : Prop :=
+forall parent child1 child2 : page ,
+  In parent (getPartitions pageRootPartition s)->
+  In child1 (getChildren parent s) ->
+  In child2 (getChildren parent s) ->
   child1 <> child2 ->
-
   disjoint (getUsedPages child1 s)(getUsedPages child2 s).
 
 (** THE ISOLATION PROPERTY BETWEEN THE KERNEL DATA AND PARTITIONS
@@ -42,11 +30,7 @@ forall parent child1 child2 : page ,
     All configuration tables of a given partition are inaccessible by all
     partitions *)
 Definition kernelDataIsolation s : Prop :=
-
-forall partition1 partition2, 
-
+forall partition1 partition2,
   In partition1 (getPartitions pageRootPartition s) ->
-
-  In partition2 (getPartitions pageRootPartition s) -> 
-
+  In partition2 (getPartitions pageRootPartition s) ->
   disjoint (getAccessibleMappedPages partition1 s) (getConfigPages partition2 s).
