proof/Isolation/ModelExclusiveFunctions.v
@@ -205,6 +205,33 @@ end.
 Definition getMappedPagesOption (pd : page) (vaList : list vaddr) s : list optionPage :=
 map (getMappedPage pd s) vaList.
 
+Definition readAccessible  (paddr : page) (idx : index) memory : option bool:=
+let entry :=  lookup paddr idx memory pageEq idxEq  in 
+  match entry with
+  | Some (PE a) => Some a.(user)
+  | Some _ => None
+  | None => None
+ end.
+
+Definition getAccessibleMappedPage pd s va: optionPage :=
+match getNbLevel  with 
+ |None => NonePage
+ |Some level =>let idxVA := getIndexOfAddr va levelMin  in 
+               match getIndirection pd va level (nbLevel - 1) s with 
+                | Some tbl => if pageDefault =? tbl
+                                   then NonePage 
+                                   else  match (readPresent tbl idxVA s.(memory)),
+                                                   (readAccessible tbl idxVA s.(memory)) with 
+                                           |Some true, Some true => match readPhyEntry tbl idxVA s.(memory)  with 
+                                                       | Some a => SomePage a
+                                                       | _ => NonePage
+                                                       end
+                                           | _, _ =>  NonePage 
+                                          end
+                | _ => NonePage
+               end
+end.
+
 (** The [getAccessibleMappedPagesOption] function Return all physical pages 
     marked as present and accessible into a partition *)
 Definition getAccessibleMappedPagesOption (pd : page) (vaList : list vaddr) s : list optionPage :=
@@ -221,6 +248,39 @@ end.
 (** The [getMappedPagesAux] function removes option type from mapped pages list *)
 Definition getMappedPagesAux (pd :page)  (vaList : list vaddr) s : list page  := 
 filterOption (getMappedPagesOption pd vaList s).
+
+Definition getFstShadow partition memory: option page:= 
+match Index.succ idxShadow1 with 
+|None => None
+|Some idx => readPhysical partition idx memory
+end.
+
+Definition readPDflag  (paddr : page) (idx : index) memory : option bool:=
+let entry :=  lookup paddr idx memory pageEq idxEq in
+  match entry with
+  | Some (VE a) => Some a.(pd)
+  | Some _ => None
+  | None => None
+ end.
+
+Definition checkChild partition level (s:state) va : bool :=
+let idxVA :=  getIndexOfAddr va levelMin in
+match getFstShadow partition s.(memory) with
+| Some sh1 =>
+   match getIndirection sh1 va level (nbLevel -1) s with
+    |Some tbl => if tbl =? pageDefault
+                    then false
+                    else match readPDflag tbl idxVA s.(memory) with
+                          | Some true => true
+                          | _ => false
+                          end
+    |None => false
+    end
+| _ => false
+end.
+
+Definition getPdsVAddr partition l1 (vaList : list vaddr) s :=
+filter (checkChild partition l1 s) vaList.
 
 (** The [getChildren] function Returns all children of a given partition *)
 Definition getChildren (partition : page) s := 
@@ -241,3 +301,244 @@ Fixpoint getPartitionAux (partitionRoot : page) (s : state) bound {struct bound}
 (** The [getPartitions] function fixes the sufficient timeout value to retrieve all partitions *)
 Definition getPartitions (root : page) s : list page  :=
 (getPartitionAux root s (nbPage+1)).
+
+Definition getMappedPages (partition : page) s : list page :=
+  match getPd partition s.(memory) with
+    |None => []
+    |Some pd => let vaList := getAllVAddrWithOffset0 in getMappedPagesAux pd vaList s
+  end.
+
+Definition getConfigTablesLinkedList partition memory: option page:= 
+match Index.succ idxShadow3 with 
+|None => None
+|Some idx => readPhysical partition idx memory
+end.
+
+Definition getSndShadow partition memory: option page:= 
+match Index.succ idxShadow2 with 
+|None => None
+|Some idx => readPhysical partition idx memory
+end.
+
+Definition getMaxIndex : option index:=
+match gt_dec tableSize 0 with
+| left x =>
+    Some
+      {|
+      i := tableSize - 1;
+      Hi := IsolationInterface.IsolationInterface.getMaxIndex_obligation_1 x |}
+| right _ => None 
+end.
+
+Fixpoint getLLPages (sh3 : page) s bound :=
+match bound with 
+|0 => []
+|S bound1 => match getMaxIndex with 
+            |None => []
+            |Some maxindex =>  match readPhysical sh3 maxindex s.(memory) with 
+                                |None => [sh3]
+                                |Some addr => if addr =? pageDefault then [sh3] else sh3 :: getLLPages addr s bound1
+                               end
+           end
+end.
+
+Definition getConfigPagesAux (partition : page) (s : state) : list page := 
+match getPd partition s.(memory),
+      getFstShadow partition s.(memory),
+      getSndShadow partition s.(memory),
+      getConfigTablesLinkedList partition s.(memory) with
+| Some pd , Some sh1, Some sh2 , Some sh3  => (getIndirections pd s)++
+                         (getIndirections sh1 s)++
+                         (getIndirections sh2 s )++
+                         (getLLPages sh3 s (nbPage+1))
+|_,_,_,_ => []
+end.
+
+Definition getConfigPages (partition : page) (s : state) :=
+partition :: (getConfigPagesAux partition s).
+
+Definition getUsedPages (partition: page) s : list page :=
+  getConfigPages partition s ++ getMappedPages partition s.
+
+
+Definition disjoint {A : Type} (l1 l2 : list A) : Prop := 
+forall x : A,  In x l1  -> ~ In x l2.
+
+Definition getAccessibleMappedPagesAux (pd :page)  (vaList : list vaddr) s : list page := 
+filterOption (getAccessibleMappedPagesOption pd vaList s).
+
+Definition getAccessibleMappedPages (partition : page) s : list page :=
+  match getPd partition s.(memory) with
+    |None => []
+    |Some pd => let vaList := getAllVAddrWithOffset0 in getAccessibleMappedPagesAux pd vaList s
+  end.
+
+Definition nextEntryIsPP table idxroot tableroot s : Prop:=
+match Index.succ idxroot with
+| Some idxsucc => match lookup table idxsucc (memory s) pageEq idxEq with
+                  | Some (PP table) => tableroot = table
+                  |_ => False
+                  end
+| _ => False
+end.
+
+Definition isPE table idx s: Prop :=
+match lookup table idx s.(memory) pageEq idxEq with
+| Some (PE _) => True
+| _ => False
+end.
+
+Definition isVE table idx s: Prop :=
+match lookup table idx s.(memory) pageEq idxEq with
+| Some (VE _) => True
+| _ => False
+end.
+
+Definition isVA table idx s: Prop := 
+match lookup table idx s.(memory) pageEq idxEq with
+| Some (VA _) => True
+| _ => False
+end.
+
+Definition isPP table idx s: Prop :=
+match lookup table idx s.(memory) pageEq idxEq with
+| Some (PP _) => True
+| _ => False
+end.
+
+Definition readVirEntry (paddr : page) (idx : index) memory : option vaddr :=
+let entry :=  lookup paddr idx memory pageEq idxEq in
+match entry with
+| Some (VE addr) => Some (va addr)
+| Some _ => None
+| None => None
+end.
+
+Definition getVirtualAddressSh1 sh1 s va: option vaddr :=
+match getNbLevel  with
+| None => None
+| Some level => let idxVA := getIndexOfAddr va levelMin in
+                match getIndirection sh1 va level (nbLevel - 1) s with
+                | Some tbl => if pageDefault =? tbl
+                              then None
+                              else readVirEntry tbl idxVA s.(memory)
+                | _ => None
+                end
+end.
+
+Definition readVirtual (paddr : page) (idx : index) memory : option vaddr :=
+let entry := lookup paddr idx memory pageEq idxEq in
+match entry with
+| Some (VA addr) => Some addr
+| Some _ => None
+| None => None
+end.
+
+Definition getVirtualAddressSh2 sh2 s va: option vaddr :=
+match getNbLevel  with 
+| None => None
+| Some level => let idxVA := getIndexOfAddr va levelMin in
+                match getIndirection sh2 va level (nbLevel - 1) s with
+                | Some tbl => if pageDefault =? tbl
+                              then None
+                              else readVirtual tbl idxVA s.(memory)
+                | _ => None
+               end
+end.
+
+Definition vaddrEq (x y : vaddr) : bool := eqList x y idxEq.
+
+Definition getParent partition memory :=
+match Index.succ idxParentDesc with
+| Some idx => readPhysical partition idx memory
+| _ => None
+end.
+
+Definition getPDFlag sh1 va s :=
+let idxVA := getIndexOfAddr va levelMin in
+match getNbLevel with
+| Some nbL =>  match getIndirection sh1 va nbL (nbLevel - 1) s with
+               | Some tbl => if tbl =? pageDefault
+                             then false
+                             else match readPDflag tbl idxVA (memory s) with
+                                  | Some true => true
+                                  | Some false => false
+                                  | None => false
+                                  end
+               | None => false
+               end
+| None => false
+end.
+
+Definition isAccessibleMappedPageInParent partition va accessiblePage s :=
+match getSndShadow partition (memory s) with
+| Some sh2 =>
+  match getVirtualAddressSh2 sh2 s va  with
+  | Some vaInParent =>
+    match getParent partition (memory s) with
+    | Some parent =>
+      match getPd parent (memory s) with
+      | Some pdParent =>
+        match getAccessibleMappedPage pdParent s vaInParent with
+        | SomePage sameAccessiblePage => accessiblePage =? sameAccessiblePage
+        | _ => false
+        end
+      | None => false
+      end
+    | None => false
+    end
+  | None => false
+  end
+| None => false
+end.
+
+Fixpoint getAncestorsAux (partition : page) memory depth : list page :=
+match depth with
+| 0 => []
+| S depth1 => match getParent partition memory with
+              | Some parent => parent :: getAncestorsAux parent memory depth1
+              | _ => []
+              end
+end.
+
+(** The [getAncestors] function fixes the sufficient timeout value to retrieve all ancestors *)
+Definition getAncestors (partition : page) s :=
+getAncestorsAux partition s.(memory) (nbPage+1).
+
+Definition isDerived partition va s :=
+match getFstShadow partition (memory s) with
+| Some sh1 =>
+  match getVirtualAddressSh1 sh1 s va with
+  | Some va0 => vaddrEq vaddrDefault va0 = false
+  | _ => False
+  end
+| None => False
+end.
+
+Definition isI table idx s : Prop :=
+match lookup table idx s.(memory) pageEq idxEq with
+| Some (I _) => True
+| _ => False
+end.
+
+Definition readIndex  (paddr : page) (idx : index) memory : option index :=
+let entry := lookup paddr idx memory pageEq idxEq in
+match entry with
+| Some (I indexValue) => Some indexValue
+| Some _ => None
+| None => None
+end.
+
+Definition isIndexValue table idx vindex s :=
+match lookup table idx (memory s) pageEq idxEq with
+| Some (I value) => value = vindex
+| _ => False
+end.
+
+
+
+
+
+
+
+
