src/model/Extraction.v
@@ -6,6 +6,15 @@ From Pip.Model.Hollow Require Import HollowModel.
 Require Extraction.
 Extraction Language Haskell.
 
+(*
+   Place the extracted AST inside the "build" folder at root
+   What ? Stop staring at me like that, even CompCert uses this. Yikes
+   https://github.com/AbsInt/CompCert/blob/master/extraction/extraction.v#L158
+*)
+Cd "build".
+
 (** EXTRACTION *)
 Module Code := ModelAgnosticCode HollowTypes HollowState HollowInterface.
 Separate Extraction Code.
+
+Cd "..".
