Makefile
@@ -1,0 +1,78 @@
+#####################################################################
+##                       Directory variables                       ##
+#####################################################################
+
+# Build directory
+BUILD_DIR=build
+
+# Sources directory
+SRC_DIR=src
+
+# Coq sources directory
+CORE_DIR=$(SRC_DIR)/core
+MODEL_DIR=$(SRC_DIR)/model
+META_MODEL_DIR=$(MODEL_DIR)/Meta
+ISOLATION_MODEL_DIR=$(MODEL_DIR)/Isolation
+HOLLOW_MODEL_DIR=$(MODEL_DIR)/Hollow
+
+# Coq proofs related directories
+PROOF_DIR=proof
+ISOLATION_PROOF_DIR=$(PROOF_DIR)/Isolation
+ISOLATION_PROOF_INVARIANTS_DIR=$(ISOLATION_PROOF_DIR)/Invariants
+
+#####################################################################
+##                      Build files variables                      ##
+#####################################################################
+
+# Coq source files
+COQ_SRC_FILES=$(foreach dir, $(CORE_DIR)\
+                             $(META_MODEL_DIR)\
+                             $(ISOLATION_MODEL_DIR)\
+                             $(HOLLOW_MODEL_DIR),\
+			$(wildcard $(dir)/*.v)\
+               )
+
+# Coq file needed for extraction
+COQ_EXTRACTION_FILE=$(MODEL_DIR)/Extraction.v
+COQ_COMPILED_EXTRACTION_FILE=$(COQ_EXTRACTION_FILE:.v=.vo)
+
+# Coq prooof files
+COQ_PROOF_FILES=$(foreach dir, $(ISOLATION_PROOF_DIR)\
+		               $(ISOLATION_PROOF_INVARIANTS_DIR),\
+			$(wildcard $(dir)/*.v)\
+		)
+
+HASKELL_EXTRACTED_FILES=Ascii.hs Datatypes.hs Extraction.hs HollowModel.hs String.hs
+HASKELL_EXTRACTED_FILES:=$(patsubst %,$(BUILD_DIR)/%, $(HASKELL_EXTRACTED_FILES))
+
+#####################################################################
+##                         Default target                          ##
+#####################################################################
+
+all : proofs
+
+#####################################################################
+##                       Compilation targets                       ##
+#####################################################################
+
+Makefile.coq: Makefile _CoqProject $(COQ_EXTRACTION_FILE) $(COQ_SRC_FILES) $(COQ_PROOF_FILES)
+	coq_makefile -f _CoqProject -o Makefile.coq $(COQ_EXTRACTION_FILE) $(COQ_SRC_FILES) $(COQ_PROOF_FILES)
+
+# All code extraction files are generated once Extraction.v is compiled
+$(HASKELL_EXTRACTED_FILES) &: coq_code_extraction ;
+
+$(BUILD_DIR):
+	mkdir -p $@
+
+proofs: Makefile.coq $(COQ_SRC_FILES) $(COQ_PROOF_FILES) $(COQ_EXTRACTION_FILES) | $(BUILD_DIR)
+	$(MAKE) -f Makefile.coq all
+
+coq_code_extraction : Makefile.coq $(COQ_EXTRACTION_FILE) | $(BUILD_DIR)
+	$(MAKE) --no-print-directory -f Makefile.coq only TGTS="$(COQ_COMPILED_EXTRACTION_FILE)" -j
+
+clean: | Makefile.coq
+	$(MAKE) -f Makefile.coq clean
+	rm -f Makefile.coq Makefile.coq.conf *~ .*.aux *.crashcoqide
+	rm -rf $(BUILD_DIR)
+
+.PHONY: all proofs coq_code_extraction clean
